.

structured_internship_machine.thy
@@ -45,11 +45,18 @@ definition cyclic_paths:: "path set" where
 
 (*-----------------EXAMPLE PATHS------------------*)
 
-definition specific_path:: "nat \<Rightarrow> STEP" where
+definition specific_path:: "path" where
 "specific_path n = \<lparr> INPUT = 0,STATE = S_1,OUT = False \<rparr>"
 
-definition two_cyclic_path:: "(nat \<Rightarrow> STEP) \<Rightarrow> bool" where
+fun specific_path_2:: "path" where
+"specific_path_2 0 = \<lparr> INPUT = 1 ,STATE = S_1,OUT = True \<rparr>"|
+"specific_path_2 n = \<lparr> INPUT = 0,STATE = S_2, OUT = True \<rparr>"
+
+definition two_cyclic_path:: "path \<Rightarrow> bool" where
 "two_cyclic_path p \<equiv> p \<in> paths \<and> (\<forall>n. INPUT(p n) = 1)"
+
+definition reachable:: "State \<Rightarrow> bool" where
+"reachable st \<equiv>  (\<exists>p\<in>paths. \<exists>n.  STATE(p n) = st)"
 
 (*-----------------HELPER LEMMAS------------------*)
 
@@ -66,6 +73,40 @@ lemma spec_path_cond1: "STATE(specific_path(0)) = S_1" using specific_path_state
 lemma spec_path_cond2: "\<forall>n. t(STATE(specific_path n),INPUT(specific_path n)) = (STATE(specific_path(Suc(n))), OUT(specific_path n))"
   by (simp add: specific_path_in specific_path_out specific_path_state)
 
+lemma specific_path_2_state: "\<forall>n > 0. STATE(specific_path_2 n) = S_2"
+proof
+  fix n::nat
+  show "0 < n \<longrightarrow> STATE (specific_path_2 n) = S_2 "
+  proof
+    assume a: "0 < n"
+    show "STATE (specific_path_2 n) = S_2"
+    by (metis a bot_nat_0.not_eq_extremum select_convs(2) specific_path_2.elims) 
+  qed
+qed
+
+lemma specific_path_2_out: "\<forall>n. OUT(specific_path_2 n) = True"
+  by (metis select_convs(3) specific_path_2.elims)
+
+lemma specific_path_2_in: "\<forall>n > 0. INPUT(specific_path_2 n) = 0"
+proof
+  fix n::nat
+  show "0 < n \<longrightarrow> INPUT(specific_path_2 n) = 0"
+  proof
+    assume a: "0 < n"
+    show "INPUT(specific_path_2 n) = 0"
+    using a gr0_conv_Suc by fastforce
+  qed
+qed
+
+(*show that spec path holds property 1 of paths*)
+lemma spec_path_2_cond1: "STATE(specific_path_2(0)) = S_1" by simp
+
+(*show that spec path holds property 2 of paths*)
+lemma spec_path_2_cond2: "\<forall>n. t(STATE(specific_path_2 n),INPUT(specific_path_2 n)) = (STATE(specific_path_2(Suc(n))), OUT(specific_path_2 n))"
+  by (smt (verit, best) select_convs(1) spec_path_2_cond1 
+specific_path_2.elims specific_path_2.simps(2) specific_path_2_out 
+specific_path_2_state t.simps(2) t.simps(3) zero_less_one)
+
 lemma two_cyclic_path_input: "\<forall>p. two_cyclic_path p \<longrightarrow> INPUT(p n) = 1" using two_cyclic_path_def by simp
 
 lemma init_is_s1 [simp]: "INITIAL_NODE \<equiv> S_1"
@@ -76,6 +117,7 @@ lemma paths_1: "\<forall>p \<in> paths. STATE(p 0) = S_1" by(simp add: paths_def
 lemma paths_2: "\<forall>p \<in> paths. t(STATE(p n),INPUT(p n)) = (STATE(p(Suc(n))), OUT(p n))"
   by (simp add: paths_def)
 
+lemma not_s_1: "s \<noteq> S_1 \<longrightarrow> s = S_2" using State.exhaust by auto
 
 lemma s2_to_s1: "\<forall>p\<in>paths. STATE(p n) = S_2 \<and> INPUT(p n) = 1 \<longrightarrow> STATE(p (Suc n)) = S_1"
   by (metis One_nat_def Pair_inject paths_2 t.simps(4))
@@ -126,6 +168,10 @@ lemma specific_in_paths: "specific_path \<in> paths"
   apply(auto simp add: paths_def spec_path_cond1 spec_path_cond2)
   done
 
+lemma specific_2_in_paths: "specific_path_2 \<in> paths"
+  apply(auto simp add: paths_def spec_path_2_cond1 spec_path_2_cond2)
+  done
+
 method interval_induct for i::nat =
   (induction i, simp, case_tac "Suc i = Suc n")
 
@@ -148,34 +194,44 @@ lemma odd_p1: "\<forall>p \<in> paths. two_cyclic_path p \<longrightarrow> STATE
 
 lemma even_p1: "\<forall>p \<in> paths. two_cyclic_path p \<longrightarrow> STATE(p (2*n)) = S_1"
   apply(auto)
-  
+  apply(induction n)
+   apply(auto simp add: paths_1)
+  apply(simp add: state_to_t_simp two_cyclic_path_input)
   done
-
-
-  
-
- 
-
-
+   
 (*-----------------MAIN LEMMAS------------------*)
 
 lemma "paths \<noteq> {}"
   using specific_in_paths by auto
 
+method machine_security = 
+(auto simp add: out_to_t_simp, ((simp add: stays_in_s_2; fail) | simp add: stays_in_s_1) )
+
 lemma security_s1_to_s2: "\<forall>p \<in> paths. STATE(p n) = S_1 \<and> INPUT(p n) > 0 \<and> (\<forall>j. j \<in> {n<..<m} \<longrightarrow> INPUT(p j) = 0) \<and> i \<in> {n<..<m} \<longrightarrow> OUT(p i) = True"
-  apply(auto simp add: out_to_t_simp)
-  apply(simp add: stays_in_s_2)
-  done
+  by machine_security
 
 lemma security_s2_to_s1: "\<forall>p \<in> paths. STATE(p n) = S_2 \<and> INPUT(p n) > 0 \<and> (\<forall>j. j \<in> {n<..<m} \<longrightarrow> INPUT(p j) = 0) \<and> i \<in> {n<..<m} \<longrightarrow> OUT(p i) = False"
-  apply(auto simp add: out_to_t_simp)
-  apply(simp add: stays_in_s_1)
-  done
+  by machine_security
 
 lemma "p \<in> paths \<and> two_cyclic_path p \<longrightarrow> (OUT(p n) \<noteq> OUT(p (Suc n))) \<and> (STATE(p n) \<noteq> STATE(p (Suc n)))"
   by (auto_two_cyclic p n)
 
+lemma two_cyclic_odd_even_prop: "\<forall>p\<in>paths. two_cyclic_path p \<longrightarrow> (odd n \<longrightarrow> STATE(p n) = S_2) \<and> (even n \<longrightarrow> STATE(p n) = S_1)"
+  by (metis dvd_mult_div_cancel even_p1 odd_p1 odd_two_times_div_two_succ)
 
+lemma all_nodes_reachable: "\<forall>s\<in>\<Sigma>. reachable s"
+  apply(auto simp add: reachable_def)
+  apply(case_tac "s = S_1")
+  using spec_path_cond1 specific_in_paths apply blast
+  using not_s_1 specific_2_in_paths specific_path_2_state by blast
+
+
+  
+  
+  
+  
+  
+  
     
  
 
