counter_machine/structured_counter_machine.thy
@@ -1,0 +1,12 @@
+theory structured_counter_machine
+  imports Main 
+begin
+
+
+(*--------------- INITIAL SETUP ---------------*)
+
+
+
+
+
+end
